Update.

src/metalogic/pred.lean
@@ -599,17 +599,17 @@ begin
 end
 
 
-def sub_formula_simp (s : instantiation) : formula → formula
+def sub (s : instantiation) : formula → formula
 | bottom := bottom
 | top := top
 | (atom n x terms) := atom n x (fun i : fin n, sub_term s (terms i))
-| (not p) := not (sub_formula_simp p)
-| (and p q) := and (sub_formula_simp p) (sub_formula_simp q)
-| (or p q) := or (sub_formula_simp p) (sub_formula_simp q)
-| (imp p q) := imp (sub_formula_simp p) (sub_formula_simp q)
-| (iff p q) := iff (sub_formula_simp p) (sub_formula_simp q)
-| (forall_ x p) := forall_ x (sub_formula_simp p)
-| (exists_ x p) := exists_ x (sub_formula_simp p)
+| (not p) := not (sub p)
+| (and p q) := and (sub p) (sub q)
+| (or p q) := or (sub p) (sub q)
+| (imp p q) := imp (sub p) (sub q)
+| (iff p q) := iff (sub p) (sub q)
+| (forall_ x p) := forall_ x (sub p)
+| (exists_ x p) := exists_ x (sub p)
 
 def sub_admits (s : instantiation) : formula → Prop
 | bottom := true
@@ -624,23 +624,23 @@ def sub_admits (s : instantiation) : formula → Prop
 | (exists_ x p) := s x = var x ∧ sub_admits p ∧ ∀ y ∈ p.free_var_set \ {x}, x ∉ (s y).all_var_set
 
 
-lemma lem_3_6_simp
+lemma lem_3_6
   (p : formula)
   (s : instantiation)
   (h1 : sub_admits s p) :
-  (sub_formula_simp s p).free_var_set = finset.bUnion p.free_var_set (fun y : string, (s y).all_var_set) :=
+  (sub s p).free_var_set = finset.bUnion p.free_var_set (fun y : string, (s y).all_var_set) :=
 begin
   induction p generalizing s,
   case formula.bottom {
-    unfold sub_formula_simp, unfold formula.free_var_set, simp only [finset.bUnion_empty]
+    unfold sub, unfold formula.free_var_set, simp only [finset.bUnion_empty]
   },
   case formula.top {
-    unfold sub_formula_simp, unfold formula.free_var_set, simp only [finset.bUnion_empty]
+    unfold sub, unfold formula.free_var_set, simp only [finset.bUnion_empty]
   },
   case formula.atom : n x terms {
     calc
-          (sub_formula_simp s (atom n x terms)).free_var_set
-        = (atom n x (fun i : fin n, sub_term s (terms i))).free_var_set : by unfold sub_formula_simp
+          (sub s (atom n x terms)).free_var_set
+        = (atom n x (fun i : fin n, sub_term s (terms i))).free_var_set : by unfold sub
     ... = finset.bUnion finset.univ (fun i : fin n, (sub_term s (terms i)).all_var_set) : by unfold formula.free_var_set
     ... = finset.bUnion finset.univ (fun i : fin n, (finset.bUnion (terms i).all_var_set (fun y : string, (s y).all_var_set))) :
           begin congr, funext, apply lem_3_4 end
@@ -650,17 +650,17 @@ begin
   },
   case formula.not : p ih {
     calc
-          (sub_formula_simp s (not p)).free_var_set
-        = (not (sub_formula_simp s p)).free_var_set : by unfold sub_formula_simp
-    ... = (sub_formula_simp s p).free_var_set : by unfold formula.free_var_set
+          (sub s (not p)).free_var_set
+        = (not (sub s p)).free_var_set : by unfold sub
+    ... = (sub s p).free_var_set : by unfold formula.free_var_set
     ... = finset.bUnion p.free_var_set (fun y : string, (s y).all_var_set) : begin unfold sub_admits at h1, exact ih s h1 end
     ... = finset.bUnion (not p).free_var_set (fun y : string, (s y).all_var_set) : by unfold formula.free_var_set
   },
   case formula.and : p q ih_p ih_q {
     calc
-          (sub_formula_simp s (and p q)).free_var_set
-        = (and (sub_formula_simp s p) (sub_formula_simp s q)).free_var_set : by unfold sub_formula_simp
-    ... = (sub_formula_simp s p).free_var_set ∪ (sub_formula_simp s q).free_var_set : by unfold formula.free_var_set
+          (sub s (and p q)).free_var_set
+        = (and (sub s p) (sub s q)).free_var_set : by unfold sub
+    ... = (sub s p).free_var_set ∪ (sub s q).free_var_set : by unfold formula.free_var_set
     ... = finset.bUnion p.free_var_set (fun y : string, (s y).all_var_set) ∪
             finset.bUnion q.free_var_set (fun y : string, (s y).all_var_set) :
           begin
@@ -672,9 +672,9 @@ begin
   },
   case formula.or : p q ih_p ih_q {
     calc
-          (sub_formula_simp s (or p q)).free_var_set
-        = (or (sub_formula_simp s p) (sub_formula_simp s q)).free_var_set : by unfold sub_formula_simp
-    ... = (sub_formula_simp s p).free_var_set ∪ (sub_formula_simp s q).free_var_set : by unfold formula.free_var_set
+          (sub s (or p q)).free_var_set
+        = (or (sub s p) (sub s q)).free_var_set : by unfold sub
+    ... = (sub s p).free_var_set ∪ (sub s q).free_var_set : by unfold formula.free_var_set
     ... = finset.bUnion p.free_var_set (fun y : string, (s y).all_var_set) ∪
             finset.bUnion q.free_var_set (fun y : string, (s y).all_var_set) :
           begin
@@ -686,9 +686,9 @@ begin
   },
   case formula.imp : p q ih_p ih_q {
     calc
-          (sub_formula_simp s (imp p q)).free_var_set
-        = (imp (sub_formula_simp s p) (sub_formula_simp s q)).free_var_set : by unfold sub_formula_simp
-    ... = (sub_formula_simp s p).free_var_set ∪ (sub_formula_simp s q).free_var_set : by unfold formula.free_var_set
+          (sub s (imp p q)).free_var_set
+        = (imp (sub s p) (sub s q)).free_var_set : by unfold sub
+    ... = (sub s p).free_var_set ∪ (sub s q).free_var_set : by unfold formula.free_var_set
     ... = finset.bUnion p.free_var_set (fun y : string, (s y).all_var_set) ∪
             finset.bUnion q.free_var_set (fun y : string, (s y).all_var_set) :
           begin
@@ -700,9 +700,9 @@ begin
   },
   case formula.iff : p q ih_p ih_q {
     calc
-          (sub_formula_simp s (iff p q)).free_var_set
-        = (iff (sub_formula_simp s p) (sub_formula_simp s q)).free_var_set : by unfold sub_formula_simp
-    ... = (sub_formula_simp s p).free_var_set ∪ (sub_formula_simp s q).free_var_set : by unfold formula.free_var_set
+          (sub s (iff p q)).free_var_set
+        = (iff (sub s p) (sub s q)).free_var_set : by unfold sub
+    ... = (sub s p).free_var_set ∪ (sub s q).free_var_set : by unfold formula.free_var_set
     ... = finset.bUnion p.free_var_set (fun y : string, (s y).all_var_set) ∪
             finset.bUnion q.free_var_set (fun y : string, (s y).all_var_set) :
           begin
@@ -715,10 +715,10 @@ begin
   case formula.forall_ : x p ih {
     unfold sub_admits at h1, cases h1, cases h1_right,
     calc
-          (sub_formula_simp s (forall_ x p)).free_var_set
-        = (forall_ x (sub_formula_simp s p)).free_var_set :
-            by unfold sub_formula_simp
-    ... = (sub_formula_simp s p).free_var_set \ {x} :
+          (sub s (forall_ x p)).free_var_set
+        = (forall_ x (sub s p)).free_var_set :
+            by unfold sub
+    ... = (sub s p).free_var_set \ {x} :
             by unfold formula.free_var_set
     ... = (finset.bUnion p.free_var_set (fun y : string, (s y).all_var_set)) \ {x} : by rewrite ih s h1_right_left
     ... = (finset.bUnion (p.free_var_set \ {x}) (fun (y : string), (s y).all_var_set)) \ {x} :
@@ -733,10 +733,10 @@ begin
   case formula.exists_ : x p ih {
     unfold sub_admits at h1, cases h1, cases h1_right,
     calc
-          (sub_formula_simp s (exists_ x p)).free_var_set
-        = (exists_ x (sub_formula_simp s p)).free_var_set :
-            by unfold sub_formula_simp
-    ... = (sub_formula_simp s p).free_var_set \ {x} :
+          (sub s (exists_ x p)).free_var_set
+        = (exists_ x (sub s p)).free_var_set :
+            by unfold sub
+    ... = (sub s p).free_var_set \ {x} :
             by unfold formula.free_var_set
     ... = (finset.bUnion p.free_var_set (fun y : string, (s y).all_var_set)) \ {x} : by rewrite ih s h1_right_left
     ... = (finset.bUnion (p.free_var_set \ {x}) (fun (y : string), (s y).all_var_set)) \ {x} :
@@ -751,65 +751,65 @@ begin
 end
 
 
-theorem thm_3_7_simp
+theorem thm_3_7
   {D : Type}
   {m : interpretation D}
   (v : valuation D)
   (s : instantiation)
   (p : formula)
   (h1 : sub_admits s p) :
-  holds D m v (sub_formula_simp s p) ↔ holds D m ((eval_term D m v) ∘ s) p :=
+  holds D m v (sub s p) ↔ holds D m ((eval_term D m v) ∘ s) p :=
 begin
   induction p generalizing s v,
   case formula.bottom {
-    unfold sub_formula_simp, unfold holds
+    unfold sub, unfold holds
   },
   case formula.top {
-    unfold sub_formula_simp, unfold holds
+    unfold sub, unfold holds
   },
   case formula.atom : n x terms {
     calc
-    holds D m v (sub_formula_simp s (atom n x terms)) ↔
-      holds D m v (atom n x (fun i : fin n, sub_term s (terms i))) : by unfold sub_formula_simp
+    holds D m v (sub s (atom n x terms)) ↔
+      holds D m v (atom n x (fun i : fin n, sub_term s (terms i))) : by unfold sub
     ... ↔ m.pred n x (fun i : fin n, eval_term D m v (sub_term s (terms i))) : by unfold holds
     ... ↔ m.pred n x (fun i : fin n, eval_term D m ((eval_term D m v) ∘ s) (terms i)) : by simp only [lem_3_5]
     ... ↔ holds D m ((eval_term D m v) ∘ s) (atom n x terms) : by unfold holds
   },
   case formula.not : p ih {
     calc
-    holds D m v (sub_formula_simp s (not p)) ↔ holds D m v (not (sub_formula_simp s p)) : by unfold sub_formula_simp
-    ... ↔ ¬ holds D m v (sub_formula_simp s p) : by unfold holds
+    holds D m v (sub s (not p)) ↔ holds D m v (not (sub s p)) : by unfold sub
+    ... ↔ ¬ holds D m v (sub s p) : by unfold holds
     ... ↔ ¬ holds D m ((eval_term D m v) ∘ s) p : begin unfold sub_admits at h1, rewrite ih s v h1 end
     ... ↔ holds D m ((eval_term D m v) ∘ s) (not p) : by unfold holds
   },
   case formula.and : p q ih_p ih_q {
     calc
-    holds D m v (sub_formula_simp s (and p q)) ↔ holds D m v (and (sub_formula_simp s p) (sub_formula_simp s q)) : by unfold sub_formula_simp
-    ... ↔ (holds D m v (sub_formula_simp s p)) ∧ (holds D m v (sub_formula_simp s q)) : by unfold holds
+    holds D m v (sub s (and p q)) ↔ holds D m v (and (sub s p) (sub s q)) : by unfold sub
+    ... ↔ (holds D m v (sub s p)) ∧ (holds D m v (sub s q)) : by unfold holds
     ... ↔ (holds D m ((eval_term D m v) ∘ s) p) ∧ (holds D m ((eval_term D m v) ∘ s) q) :
         begin unfold sub_admits at h1, cases h1, rewrite ih_p s v h1_left, rewrite ih_q s v h1_right end
     ... ↔ holds D m ((eval_term D m v) ∘ s) (and p q) : by unfold holds
   },
   case formula.or : p q ih_p ih_q {
     calc
-    holds D m v (sub_formula_simp s (or p q)) ↔ holds D m v (or (sub_formula_simp s p) (sub_formula_simp s q)) : by unfold sub_formula_simp
-    ... ↔ (holds D m v (sub_formula_simp s p)) ∨ (holds D m v (sub_formula_simp s q)) : by unfold holds
+    holds D m v (sub s (or p q)) ↔ holds D m v (or (sub s p) (sub s q)) : by unfold sub
+    ... ↔ (holds D m v (sub s p)) ∨ (holds D m v (sub s q)) : by unfold holds
     ... ↔ (holds D m ((eval_term D m v) ∘ s) p) ∨ (holds D m ((eval_term D m v) ∘ s) q) :
         begin unfold sub_admits at h1, cases h1, rewrite ih_p s v h1_left, rewrite ih_q s v h1_right end
     ... ↔ holds D m ((eval_term D m v) ∘ s) (or p q) : by unfold holds
   },
   case formula.imp : p q ih_p ih_q {
     calc
-    holds D m v (sub_formula_simp s (imp p q)) ↔ holds D m v (imp (sub_formula_simp s p) (sub_formula_simp s q)) : by unfold sub_formula_simp
-    ... ↔ (holds D m v (sub_formula_simp s p)) → (holds D m v (sub_formula_simp s q)) : by unfold holds
+    holds D m v (sub s (imp p q)) ↔ holds D m v (imp (sub s p) (sub s q)) : by unfold sub
+    ... ↔ (holds D m v (sub s p)) → (holds D m v (sub s q)) : by unfold holds
     ... ↔ (holds D m ((eval_term D m v) ∘ s) p) → (holds D m ((eval_term D m v) ∘ s) q) :
         begin unfold sub_admits at h1, cases h1, rewrite ih_p s v h1_left, rewrite ih_q s v h1_right end
     ... ↔ holds D m ((eval_term D m v) ∘ s) (imp p q) : by unfold holds
   },
   case formula.iff : p q ih_p ih_q {
     calc
-    holds D m v (sub_formula_simp s (iff p q)) ↔ holds D m v (iff (sub_formula_simp s p) (sub_formula_simp s q)) : by unfold sub_formula_simp
-    ... ↔ ((holds D m v (sub_formula_simp s p)) ↔ (holds D m v (sub_formula_simp s q))) : by unfold holds
+    holds D m v (sub s (iff p q)) ↔ holds D m v (iff (sub s p) (sub s q)) : by unfold sub
+    ... ↔ ((holds D m v (sub s p)) ↔ (holds D m v (sub s q))) : by unfold holds
     ... ↔ ((holds D m ((eval_term D m v) ∘ s) p) ↔ (holds D m ((eval_term D m v) ∘ s) q)) :
         begin unfold sub_admits at h1, cases h1, rewrite ih_p s v h1_left, rewrite ih_q s v h1_right end
     ... ↔ holds D m ((eval_term D m v) ∘ s) (iff p q) : by unfold holds
@@ -818,9 +818,9 @@ begin
     begin
       unfold sub_admits at h1, cases h1, cases h1_right,
       calc
-            holds D m v (sub_formula_simp s (forall_ x p))
-          ↔ holds D m v (forall_ x (sub_formula_simp s p)) : by unfold sub_formula_simp
-      ... ↔ (∀ a : D, holds D m ([x ↦ a] v) (sub_formula_simp s p)) : by unfold holds
+            holds D m v (sub s (forall_ x p))
+          ↔ holds D m v (forall_ x (sub s p)) : by unfold sub
+      ... ↔ (∀ a : D, holds D m ([x ↦ a] v) (sub s p)) : by unfold holds
       ... ↔ (∀ a : D, holds D m (eval_term D m ([x ↦ a] v) ∘ s) p) :
             begin
               apply forall_congr, intros a,
@@ -864,9 +864,9 @@ begin
     begin
       unfold sub_admits at h1, cases h1, cases h1_right,
       calc
-            holds D m v (sub_formula_simp s (exists_ x p))
-          ↔ holds D m v (exists_ x (sub_formula_simp s p)) : by unfold sub_formula_simp
-      ... ↔ (∃ a : D, holds D m ([x ↦ a] v) (sub_formula_simp s p)) : by unfold holds
+            holds D m v (sub s (exists_ x p))
+          ↔ holds D m v (exists_ x (sub s p)) : by unfold sub
+      ... ↔ (∃ a : D, holds D m ([x ↦ a] v) (sub s p)) : by unfold holds
       ... ↔ (∃ a : D, holds D m (eval_term D m ([x ↦ a] v) ∘ s) p) :
             begin
               apply exists_congr, intros a,
@@ -909,16 +909,16 @@ begin
 end
 
 
-theorem cor_3_8_simp
+theorem cor_3_8
   (p : formula)
   (s : instantiation)
   (h1 : sub_admits s p)
   (h2 : is_valid p) :
-  is_valid (sub_formula_simp s p) :=
+  is_valid (sub s p) :=
 begin
   unfold is_valid at *,
   intros D m v,
-  simp only [thm_3_7_simp v s p h1], apply h2
+  simp only [thm_3_7 v s p h1], apply h2
 end
 
 
@@ -1024,11 +1024,11 @@ theorem is_valid_pred_2
   (x : string)
   (t : term)
   (h1 : sub_admits (sub_single_var x t) p) :
-  is_valid ((forall_ x p).imp (sub_formula_simp (sub_single_var x t) p)) :=
+  is_valid ((forall_ x p).imp (sub (sub_single_var x t) p)) :=
 begin
   unfold is_valid, unfold holds,
   intros D m v h2,
-  simp only [thm_3_7_simp v (sub_single_var x t) p h1],
+  simp only [thm_3_7 v (sub_single_var x t) p h1],
   have s1 : ((eval_term D m v) ∘ (sub_single_var x t)) = ([x ↦ (eval_term D m v t)] v),
     apply funext, intros y, unfold function.comp, unfold sub_single_var,
     by_cases y = x,
